<?xml version="1.0"?>


<!DOCTYPE rdf:RDF [
    <!ENTITY owl "http://www.w3.org/2002/07/owl#" >
    <!ENTITY odip "http://odip.opendatasupport.eu/" >
    <!ENTITY xsd "http://www.w3.org/2001/XMLSchema#" >
    <!ENTITY rdfs "http://www.w3.org/2000/01/rdf-schema#" >
    <!ENTITY rdf "http://www.w3.org/1999/02/22-rdf-syntax-ns#" >
]>


<rdf:RDF xmlns="http://opendatasupport.eu/ontology/DCAT-AP-ext#"
     xml:base="http://opendatasupport.eu/ontology/DCAT-AP-ext"
     xmlns:rdfs="http://www.w3.org/2000/01/rdf-schema#"
     xmlns:owl="http://www.w3.org/2002/07/owl#"
     xmlns:xsd="http://www.w3.org/2001/XMLSchema#"
     xmlns:rdf="http://www.w3.org/1999/02/22-rdf-syntax-ns#"
     xmlns:odip="http://odip.opendatasupport.eu/">
    <owl:Ontology rdf:about="http://opendatasupport.eu/ontology/harmonisation.owl">
        <owl:imports rdf:resource="http://www.w3.org/ns/dcat"/>
    </owl:Ontology>
    


    <!-- 
    ///////////////////////////////////////////////////////////////////////////////////////
    //
    // Annotation properties
    //
    ///////////////////////////////////////////////////////////////////////////////////////
     -->

    


    <!-- 
    ///////////////////////////////////////////////////////////////////////////////////////
    //
    // Datatypes
    //
    ///////////////////////////////////////////////////////////////////////////////////////
     -->

    


    <!-- 
    ///////////////////////////////////////////////////////////////////////////////////////
    //
    // Object Properties
    //
    ///////////////////////////////////////////////////////////////////////////////////////
     -->

    


    <!-- http://opendatasupport.eu/ontology/harmonisation.owl#raw_catalog -->

    <owl:ObjectProperty rdf:about="http://opendatasupport.eu/ontology/harmonisation.owl#raw_catalog">
        <rdfs:comment>relates the harmonized catalog with the original source catalog</rdfs:comment>
        <rdfs:range rdf:resource="http://www.w3.org/ns/dcat#Catalog"/>
        <rdfs:domain rdf:resource="http://www.w3.org/ns/dcat#Catalog"/>
    </owl:ObjectProperty>
    


    <!-- http://opendatasupport.eu/ontology/harmonisation.owl#raw_dataset -->

    <owl:ObjectProperty rdf:about="http://opendatasupport.eu/ontology/harmonisation.owl#raw_dataset">
        <rdfs:comment>relates the harmonized dataset in a harmonized catalog with the original dataset in the original catalog</rdfs:comment>
        <rdfs:range rdf:resource="http://purl.org/dc/dcmitype/Dataset"/>
        <rdfs:subPropertyOf rdf:resource="&owl;topObjectProperty"/>
        <rdfs:domain rdf:resource="http://www.w3.org/ns/dcat#Dataset"/>
    </owl:ObjectProperty>
    


    <!-- 
    ///////////////////////////////////////////////////////////////////////////////////////
    //
    // Data properties
    //
    ///////////////////////////////////////////////////////////////////////////////////////
     -->

    


    <!-- http://opendatasupport.eu/ontology/harmonisation.owl#content_hash -->

    <owl:DatatypeProperty rdf:about="http://opendatasupport.eu/ontology/harmonisation.owl#content_hash">
        <rdfs:comment>a system generated hash value that encodes the content of the dataset as a hash value. This is used to identify if the dataset content is changed over time.</rdfs:comment>
        <rdfs:domain rdf:resource="http://www.w3.org/ns/dcat#Dataset"/>
        <rdfs:range rdf:resource="&xsd;int"/>
    </owl:DatatypeProperty>
    


    <!-- http://opendatasupport.eu/ontology/harmonisation.owl#harvest_date -->

    <owl:DatatypeProperty rdf:about="http://opendatasupport.eu/ontology/harmonisation.owl#harvest_date">
        <rdfs:comment>The dateTime indicating when the harvesting of a catalog or dataset in a catalog has happened.</rdfs:comment>
        <rdfs:domain rdf:resource="http://www.w3.org/ns/dcat#Dataset"/>
        <rdfs:range rdf:resource="&xsd;dateTime"/>
        <rdfs:domain rdf:resource="http://www.w3.org/ns/dcat#Catalog"/>
    </owl:DatatypeProperty>
</rdf:RDF>



<!-- Generated by the OWL API (version 3.3.1957) http://owlapi.sourceforge.net -->

